Add disk.Get() to use implicit disk as object
The package-level Read/Write/... methods are now redundant and
deprecated.

This commit ports the wal example to this new style.  We should port the
remaining examples to use a disk object instead (which a closed program
can get via the global variable using disk.Get() in Goose and
disk.Init(d) as setup from outside Goose code).

machine/disk/disk.go
@@ -91,22 +91,35 @@ func Init(d Disk) {
 	implicitDisk = d
 }
 
+// Get returns the previously-initialized global disk
+func Get() Disk {
+	return implicitDisk
+}
+
 // Read (see the Disk documentation)
+//
+// Deprecated: use Get() and the Disk method
 func Read(a uint64) Block {
 	return implicitDisk.Read(a)
 }
 
 // Write (see the Disk documentation)
+//
+// Deprecated: use Get() and the Disk method
 func Write(a uint64, v Block) {
 	implicitDisk.Write(a, v)
 }
 
 // Size (see the Disk documentation)
+//
+// Deprecated: use Get() and the Disk method
 func Size() uint64 {
 	return implicitDisk.Size()
 }
 
 // Barrier (see the Disk documentation)
+//
+// Deprecated: use Get() and the Disk method
 func Barrier() {
 	implicitDisk.Barrier()
 }
